Isa/Exp.v
@@ -6,31 +6,45 @@ Set Implicit Arguments.
 (** * Expressions *)
 
 (* Module Type Expressions. *)
-(** Assume expressions. We could pack them into a module type, but at the moment 
+(** Assume expressions. We could pack them into a module type, but at the moment
    this would not buy as anything. Packing things in module types only is interesting
    if the module types are instantiated; and expression are not in this development *)
 
   Definition binop : Set := nat.
   Definition option_lift A B C (f:A -> B -> C) := fun x y => Some (f x y).
-  Definition binop_eval (o:binop) := 
+  Definition binop_eval (o:binop) :=
     match o with
       | 0 => option_lift Peano.plus
       | 1 => option_lift minus
       | 2 => option_lift mult
       | _ => fun _ _ => None
     end.
-  
 
-  Inductive exp := 
+
+  Inductive exp :=
      Con : val -> exp
    | Var : var -> exp
    | BinOp : binop -> exp -> exp -> exp.
+
+  Inductive isVar : exp -> Prop :=
+    IisVar v : isVar (Var v).
+
+  Instance isVar_dec e : Computable (isVar e).
+  Proof.
+    destruct e; try dec_solve.
+  Qed.
+
+  Definition getVar (e:exp) :=
+    match e with
+      | Var y => y
+      | _ => 0
+    end.
 
   Fixpoint exp_eval (E:onv val) (e:exp) : option val :=
     match e with
       | Con v => Some v
       | Var x => E x
-      | BinOp o e1 e2 => mdo v1 <- exp_eval E e1; 
+      | BinOp o e1 e2 => mdo v1 <- exp_eval E e1;
                         mdo v2 <- exp_eval E e2;
                         binop_eval o v1 v2
     end.
@@ -39,23 +53,23 @@ Set Implicit Arguments.
   | conOfType ET v t : expOfType ET (Con v) t
   | varOfType ET x t : ET x = Some t -> expOfType ET (Var x) t.
 
-  Lemma expOfType_subEnv 
+  Lemma expOfType_subEnv
     : forall ET ET' e t, subEnv ET' ET -> expOfType ET' e t -> expOfType ET e t.
   Proof.
-    intros; destruct e; inv H0; eauto using expOfType.    
+    intros; destruct e; inv H0; eauto using expOfType.
   Qed.
 
-  Lemma exp_type_soundness : 
+  Lemma exp_type_soundness :
     forall ET E e t v, expOfType ET e t ->
-                       envOfType E ET -> 
+                       envOfType E ET ->
                        exp_eval E e = Some v ->
                        valOfType v t.
   Proof.
-    intros. destruct e,t; eexists; firstorder using valOfType. 
+    intros. destruct e,t; eexists; firstorder using valOfType.
   Qed.
 
-  Lemma exp_eval_typed_eq 
-    : forall ET E E' e t, typed_eq ET E E' -> expOfType ET e t 
+  Lemma exp_eval_typed_eq
+    : forall ET E E' e t, typed_eq ET E E' -> expOfType ET e t
       -> exp_eval E e = exp_eval E' e.
   Proof.
     intros. destruct e; inv H0; simpl; eauto.
@@ -64,9 +78,9 @@ Set Implicit Arguments.
   Inductive live_exp_sound : exp -> set var -> Prop :=
   | conLiveSound v lv : live_exp_sound (Con v) lv
   | varLiveSound x lv : x ∈ lv -> live_exp_sound (Var x) lv
-  | binopLiveSound o e1 e2 lv : 
+  | binopLiveSound o e1 e2 lv :
       live_exp_sound e1 lv ->
-      live_exp_sound e2 lv -> 
+      live_exp_sound e2 lv ->
       live_exp_sound (BinOp o e1 e2) lv.
 
   Instance live_exp_sound_dec e lv
@@ -77,23 +91,23 @@ Set Implicit Arguments.
     - edestruct IHe1, IHe2; dec_solve.
   Defined.
 
-  Lemma live_exp_sound_incl 
+  Lemma live_exp_sound_incl
     : forall e lv lv', lv' ⊆ lv -> live_exp_sound e lv' -> live_exp_sound e lv.
   Proof.
     intros; general induction H0; econstructor; eauto.
   Qed.
 
-  Fixpoint freeVars (e:exp) : set var := 
+  Fixpoint freeVars (e:exp) : set var :=
     match e with
       | Con _ => ∅
       | Var v => {v}
       | BinOp o e1 e2 => freeVars e1 ∪ freeVars e2
     end.
-    
+
   Lemma live_freeVars
     : forall e, live_exp_sound e (freeVars e).
   Proof.
-    intros. general induction e; simpl; econstructor. cset_tac; eauto. 
+    intros. general induction e; simpl; econstructor. cset_tac; eauto.
     eapply live_exp_sound_incl; eauto. cset_tac; intuition.
     eapply live_exp_sound_incl; eauto. cset_tac; intuition.
   Qed.
@@ -113,26 +127,26 @@ Set Implicit Arguments.
   : Equivalence (option_R R).
   Proof.
     econstructor.
-    - hnf; intros. 
+    - hnf; intros.
   Admitted.
-            
-  Definition agreed_on X `{OrderedType X} Y R `{Equivalence _ R} := 
+
+  Definition agreed_on X `{OrderedType X} Y R `{Equivalence _ R} :=
     @agree_on X _ (option Y) (option_R R) _.
 *)
-  Lemma exp_eval_live 
-    : forall e lv E E', live_exp_sound e lv -> agree_on eq lv E E' -> 
+  Lemma exp_eval_live
+    : forall e lv E E', live_exp_sound e lv -> agree_on eq lv E E' ->
       exp_eval E e = exp_eval E' e.
   Proof.
     intros. general induction e; inv H; simpl; eauto.
-    erewrite IHe1, IHe2; eauto. 
+    erewrite IHe1, IHe2; eauto.
   Qed.
 
-  Global Instance eval_exp_ext 
+  Global Instance eval_exp_ext
   : Proper (@feq _ _ eq ==> eq ==> eq) exp_eval.
   Proof.
     unfold Proper, respectful; intros; subst.
     general induction y0; simpl; eauto.
-    erewrite IHy0_1, IHy0_2; eauto. 
+    erewrite IHy0_1, IHy0_2; eauto.
   Qed.
 
   Definition var_to_exp : forall x:var, exp := Var.
@@ -140,7 +154,7 @@ Set Implicit Arguments.
      exp_eval M (var_to_exp x) = M x.
   Proof.
     reflexivity.
-  Qed.  
+  Qed.
 
   Fixpoint rename_exp (ϱ:env var) (s:exp) : exp :=
     match s with
@@ -149,22 +163,22 @@ Set Implicit Arguments.
       | BinOp o e1 e2 => BinOp o (rename_exp ϱ e1) (rename_exp ϱ e2)
     end.
 
-  Lemma rename_exp_comp e ϱ ϱ' 
+  Lemma rename_exp_comp e ϱ ϱ'
   : rename_exp ϱ (rename_exp ϱ' e) = rename_exp (ϱ' ∘ ϱ) e.
   Proof.
     unfold comp. general induction e; simpl; eauto.
     f_equal; eauto.
   Qed.
 
-  Lemma rename_exp_ext 
+  Lemma rename_exp_ext
     : forall e (ϱ ϱ':env var), feq (R:=eq) ϱ ϱ' -> rename_exp ϱ e = rename_exp ϱ' e.
   Proof.
     intros. general induction e; simpl; eauto. f_equal; eauto.
   Qed.
 
 
-  Lemma rename_exp_freeVars 
-  : forall e ϱ `{Proper _ (_eq ==> _eq) ϱ}, 
+  Lemma rename_exp_freeVars
+  : forall e ϱ `{Proper _ (_eq ==> _eq) ϱ},
       freeVars (rename_exp ϱ e) ⊆ lookup_set ϱ (freeVars e).
   Proof.
     intros. general induction e; simpl; cset_tac; intuition.
@@ -190,14 +204,14 @@ Set Implicit Arguments.
       | BinOp o e1 e2 => BinOp o (subst_exp ϱ e1) (subst_exp ϱ e2)
     end.
 
-  Lemma subst_exp_comp e ϱ ϱ' 
+  Lemma subst_exp_comp e ϱ ϱ'
   : subst_exp ϱ (subst_exp ϱ' e) = subst_exp (fun x => subst_exp ϱ (ϱ' x)) e.
   Proof.
     general induction e; simpl; eauto.
     f_equal; eauto.
   Qed.
 
-  Lemma subst_exp_ext 
+  Lemma subst_exp_ext
     : forall e (ϱ ϱ':env exp), feq (R:=eq) ϱ ϱ' -> subst_exp ϱ e = subst_exp ϱ' e.
   Proof.
     intros. general induction e; simpl; eauto. f_equal; eauto.
@@ -216,26 +230,26 @@ Set Implicit Arguments.
       inverse_on (freeVars e) ϱ ϱ'
       -> alpha_exp ϱ ϱ' e (rename_exp ϱ e).
   Proof.
-    intros. induction e; simpl; eauto using alpha_exp. 
+    intros. induction e; simpl; eauto using alpha_exp.
     econstructor; eauto. eapply H; eauto. simpl; cset_tac; eauto.
-    simpl in *. econstructor. 
+    simpl in *. econstructor.
     eapply IHe1. eapply inverse_on_incl; eauto. cset_tac; intuition.
     eapply IHe2. eapply inverse_on_incl; eauto. cset_tac; intuition.
   Qed.
-  
+
   Lemma alpha_exp_refl : forall e, alpha_exp id id e e.
   Proof.
     intros; induction e; eauto using alpha_exp.
   Qed.
-  
+
   Lemma alpha_exp_sym : forall ϱ ϱ' e e', alpha_exp ϱ ϱ' e e' -> alpha_exp ϱ' ϱ e' e.
   Proof.
     intros. general induction H; eauto using alpha_exp.
   Qed.
 
-  Lemma alpha_exp_trans 
+  Lemma alpha_exp_trans
   : forall ϱ1 ϱ1' ϱ2 ϱ2' s s' s'',
-      alpha_exp ϱ1 ϱ1' s s' 
+      alpha_exp ϱ1 ϱ1' s s'
       -> alpha_exp ϱ2 ϱ2' s' s''
       -> alpha_exp (ϱ1 ∘ ϱ2) (ϱ2' ∘ ϱ1') s s''.
   Proof.
@@ -244,7 +258,7 @@ Set Implicit Arguments.
     + inversion H1. subst x0 ϱ0 ϱ'0 s''. econstructor; unfold comp; congruence.
     + inversion H1. subst ϱ0 ϱ'0 o0 e0 e3 s''. econstructor; eauto.
   Qed.
-  
+
   Lemma alpha_exp_inverse_on
     : forall ϱ ϱ' s t, alpha_exp ϱ ϱ' s t -> inverse_on (freeVars s) ϱ ϱ'.
   Proof.
@@ -254,7 +268,7 @@ Set Implicit Arguments.
     + simpl. eapply inverse_on_union; eauto.
   Qed.
 
-  Lemma alpha_exp_agree_on_morph 
+  Lemma alpha_exp_agree_on_morph
   : forall f g ϱ ϱ' s t,
       alpha_exp ϱ ϱ' s t
       -> agree_on _eq (lookup_set ϱ (freeVars s)) g ϱ'
@@ -262,11 +276,11 @@ Set Implicit Arguments.
       -> alpha_exp f g s t.
   Proof.
     intros. general induction H; eauto using alpha_exp.
-    econstructor.     
+    econstructor.
     + rewrite <- H. eapply H2; simpl; cset_tac; eauto.
     + rewrite <- H0. eapply H1. set_tac. eexists x; simpl; cset_tac; eauto.
       intuition.
-    + simpl in *. econstructor. 
+    + simpl in *. econstructor.
       - eapply IHalpha_exp1; eauto.
         eapply agree_on_incl; eauto. eapply lookup_set_incl; intuition.
         eapply agree_on_incl; eauto. eapply union_subset_1; intuition.
@@ -280,12 +294,12 @@ Set Implicit Arguments.
   Inductive notOccur : set var -> exp -> Prop :=
   | conNotOccur D v : notOccur D (Con v)
   | varNotOccur D x : x ∉ D -> notOccur D (Var x)
-  | binopNotOccur D o e1 e2 : 
+  | binopNotOccur D o e1 e2 :
       notOccur D e1 ->
       notOccur D e2 ->
       notOccur D (BinOp o e1 e2).
 
-  Lemma notOccur_freeVars 
+  Lemma notOccur_freeVars
   : forall D e, notOccur D e <-> D ∩ freeVars e [=] ∅.
   Proof.
     intros. general induction e; simpl; split; intros; eauto using notOccur.
@@ -298,28 +312,28 @@ Set Implicit Arguments.
       eapply IHe2. cset_tac; intuition. eapply H; eauto.
   Qed.
 
-  Lemma notOccur_antitone 
+  Lemma notOccur_antitone
   : forall D D' e, D' ⊆ D -> notOccur D e -> notOccur D' e.
   Proof.
     intros. general induction H0; eauto using notOccur.
   Qed.
 
-  
-  Lemma alpha_exp_morph 
+
+  Lemma alpha_exp_morph
   : forall (ϱ1 ϱ1' ϱ2 ϱ2':env var) e e',
-      @feq _ _ eq ϱ1  ϱ1' 
-      -> @feq _ _ eq ϱ2 ϱ2' 
-      -> alpha_exp ϱ1 ϱ2 e e' 
+      @feq _ _ eq ϱ1  ϱ1'
+      -> @feq _ _ eq ϱ2 ϱ2'
+      -> alpha_exp ϱ1 ϱ2 e e'
       -> alpha_exp ϱ1' ϱ2' e e'.
   Proof.
     intros. general induction H1; eauto using alpha_exp.
-    econstructor. 
+    econstructor.
     + rewrite <- H1; eauto.
     + rewrite <- H2; eauto.
   Qed.
 
 Inductive expLt : exp -> exp -> Prop :=
-| expLtCon c c' 
+| expLtCon c c'
   : _lt c c'
     -> expLt (Con c) (Con c')
 | expLtConVar c v
@@ -344,15 +358,15 @@ Inductive expLt : exp -> exp -> Prop :=
 
 Instance expLt_irr : Irreflexive expLt.
 hnf; intros; unfold complement.
-- induction x; inversion 1; subst; eauto using StrictOrder_Irreflexive. 
+- induction x; inversion 1; subst; eauto using StrictOrder_Irreflexive.
   + eapply (StrictOrder_Irreflexive _ H2).
   + eapply (StrictOrder_Irreflexive _ H2).
   + eapply (StrictOrder_Irreflexive _ H1).
 Qed.
 
 Instance expLt_trans : Transitive expLt.
-hnf; intros. 
-general induction H; invt expLt; eauto using expLt. 
+hnf; intros.
+general induction H; invt expLt; eauto using expLt.
 - econstructor. eapply StrictOrder_Transitive; eauto.
 - econstructor. eapply StrictOrder_Transitive; eauto.
 - econstructor; eauto. transitivity o'; eauto.
@@ -365,21 +379,21 @@ Notation "'Compare' x 'next' y" :=
   end) (at level 100).
 
 Fixpoint exp_cmp (e e':exp) :=
-  match e, e' with 
+  match e, e' with
     | Con c, Con c' => _cmp c c'
     | Con _, _ => Lt
     | Var v, Var v' => _cmp v v'
     | Var v, BinOp _ _ _ => Lt
-    | BinOp o e1 e2, BinOp o' e1' e2' => 
-      Compare _cmp o o' next 
-      Compare exp_cmp e1 e1' next 
+    | BinOp o e1 e2, BinOp o' e1' e2' =>
+      Compare _cmp o o' next
+      Compare exp_cmp e1 e1' next
       Compare exp_cmp e2 e2' next Eq
     | _, _ => Gt
   end.
 
 Instance StrictOrder_expLt : OrderedType.StrictOrder expLt eq.
 econstructor.
-eapply expLt_trans. 
+eapply expLt_trans.
 intros. intro. eapply expLt_irr. rewrite H0 in H.
 eapply H.
 Qed.
@@ -388,11 +402,11 @@ Instance OrderedType_exp : OrderedType exp :=
  { _eq := eq;
   _lt := expLt;
   _cmp := exp_cmp}.
-intros. 
+intros.
 general induction x; destruct y; simpl; try now (econstructor; eauto using expLt).
-pose proof (_compare_spec v v0). 
+pose proof (_compare_spec v v0).
 inv H; now (econstructor; eauto using expLt).
-pose proof (_compare_spec v v0). 
+pose proof (_compare_spec v v0).
 inv H; now (econstructor; eauto using expLt).
 pose proof (_compare_spec b b0).
 specialize (IHx1 y1). specialize (IHx2 y2).
@@ -405,7 +419,7 @@ Defined.
 
 (* End Expressions. *)
 
-(* 
+(*
 *** Local Variables: ***
 *** coq-load-path: (("../" "Lvc")) ***
 *** End: ***
